docs/evidence/2026-09-03_bug087-paniktext/probes/shapes/sub/sub.go
@@ -1,0 +1,5 @@
+package sub
+
+type T struct{ v int }
+
+func (t T) Val() int { return t.v }
